

- (a) i All the values of  $\alpha_i$  are non-negative ( $\alpha_i \geq 0$ ) and their summation is 1. ( $\sum_{i=1}^n \alpha_i = 1$ )  
These two features make  $\alpha$  able to be considered as probability distribution
- ii When the query vector  $q$  is significantly more aligned with the key vector  $k_j$  than any other key vector  $k_i$  ( $i \neq j$ ), resulting in a much larger  $k_j^T q$ , the distribution of  $\alpha$  concentrates almost all of its weight on the single component  $\alpha_j$
- iii When  $\alpha_j \simeq 1$  and  $\alpha_i \simeq 0$  ( $i \neq j$ ),  $c = \frac{n}{j-1} \sum_{i=1}^n \alpha_i \simeq \sum_{i=1}^n \alpha_i$
- iv If the query is highly similar to a specific key, the attention mechanism acts as a copying, or lookup system. It allows the model to dynamically focus on a single information from a larger set of inputs and pass its value directly to the output

(b) i  $A = \begin{bmatrix} d_1 & d_2 & \dots & d_m \end{bmatrix}$ ,  $M = A \cdot A^T$   $M_s = M(v_a + v_b) = M v_a + M v_b$

①  $M v_a = (A A^T) (A c) = \underbrace{A (A^T A)}_c = A c = v_a$

$$A^T A = \begin{bmatrix} -a^T & -a^T \\ \vdots & \vdots \\ -a^T & -a^T \end{bmatrix} \begin{bmatrix} d_1 & \dots & d_m \\ b_1 & \dots & b_p \end{bmatrix} = \begin{bmatrix} a^T a_1 & \dots & a^T a_m \\ \vdots & \vdots & \vdots \\ a^T a_1 & \dots & a^T a_m \end{bmatrix} = I \quad (\because a^T a_j = \begin{cases} 1 & (i=j) \\ 0 & (i \neq j) \end{cases})$$

$$v_a = c_1 a_1 + c_2 a_2 + \dots + c_m a_m = A \cdot \begin{bmatrix} c_1 \\ \vdots \\ c_m \end{bmatrix} = A \cdot c$$

②  $M v_b = A A^T B c' = 0$

$$A^T B = \begin{bmatrix} -a^T & -a^T \\ \vdots & \vdots \\ -a^T & -a^T \end{bmatrix} \begin{bmatrix} b_1 & \dots & b_p \\ b_1 & \dots & b_p \end{bmatrix} = \begin{bmatrix} a^T b_1 & \dots & a^T b_p \\ \vdots & \vdots & \vdots \\ a^T b_1 & \dots & a^T b_p \end{bmatrix} = 0 \quad (\because a^T b_j = 0 \text{ for all } i, j)$$

by ①, ②,  $M_s = M(v_a + v_b) = M v_a + M v_b = v_a + 0 = v_a$ .

ii  $c \simeq \frac{1}{2} (v_a + v_b) \rightarrow \alpha_a \simeq 0.5, \alpha_b \simeq 0.5, \alpha_i (i \neq a, b) \simeq 0$

Let  $q = k_a + k_b$

$$\begin{pmatrix} k_a^T q = k_a^T (k_a + k_b) = 1 + 0 = 1 \\ k_b^T q = k_b^T (k_a + k_b) = 0 + 1 = 1 \\ k_i^T q = k_i^T (k_a + k_b) = 0 + 0 = 0 \end{pmatrix} \quad \alpha_a = \frac{e^1}{2e^1 + \sum_{i \neq a, b} e^0} \neq \frac{1}{2}$$

using hint, let  $q = c \cdot (k_a + k_b)$  which  $c$  is extremely large scalar value

$$\alpha_a = \alpha_b = \frac{e^c}{2e^c + (n-2)e^0} \simeq \frac{1}{2}.$$

(c) i  $\Sigma_{\tilde{a}} = \alpha I$  ( $\alpha$ : vanishingly small)  $\Rightarrow \tilde{k}_{\tilde{a}} \simeq \mu_{\tilde{a}}$   
 so, let  $\tilde{g} = C(\mu_a + \mu_b)$ ,  $\tilde{k}_{\tilde{a}}^T \tilde{g} \simeq \mu_{\tilde{a}}^T \tilde{g}$ .  $\therefore C \simeq \frac{1}{2}(\mu_a + \mu_b)$

ii let's rewrite score  $S_a = \tilde{k}_{\tilde{a}}^T \tilde{g} = C(\tilde{k}_{\tilde{a}}^T \mu_a + \tilde{k}_{\tilde{a}}^T \mu_b)$   
 $\text{Var}[S_a] = \text{Var}[\tilde{k}_{\tilde{a}}^T \tilde{g}] = \tilde{g}^T \text{Cov}[\tilde{k}_{\tilde{a}}^T] \tilde{g} = C^2(\mu_a + \mu_b)^T (\alpha I + \frac{1}{2} \mu_a \mu_a^T)(\mu_a + \mu_b)$   
 $= C^2(\alpha \mu_a^T \mu_a + \frac{1}{2} \mu_a^T \mu_a \mu_a^T \mu_a + \alpha \mu_a^T \mu_b + \frac{1}{2} \mu_a^T \mu_a \mu_a^T \mu_b$   
 $+ \alpha \mu_b^T \mu_a + \frac{1}{2} \mu_b^T \mu_a \mu_a^T \mu_a + \alpha \mu_b^T \mu_b + \frac{1}{2} \mu_b^T \mu_a \mu_a^T \mu_b)$   
 $(\mu_a^T \mu_a = \mu_b^T \mu_b = 1, \mu_a^T \mu_b = \mu_b^T \mu_a = 0)$   
 $= C^2(2\alpha + \frac{1}{2}) \simeq \frac{C^2}{2}$

$$\text{Var}[S_b] = \tilde{g}^T \text{Cov}[\tilde{k}_{\tilde{b}}^T] \tilde{g} = C^2(\mu_a + \mu_b)^T \alpha I (\mu_a + \mu_b) = 2\alpha C^2 \simeq 0$$

$\therefore C = v_1 a_1 + v_2 a_2 + \dots + v_m a_m$  isn't a stable mean

and single-head attention is not robust for this kind of noise.

(d) i let  $\tilde{g}_1 = \mu_a$ ,  $\tilde{g}_2 = \mu_b$   
 in head 1,  $S_{1,a} = \tilde{k}_{1,\tilde{a}}^T \mu_a \simeq \mu_{1,\tilde{a}}^T \mu_a = 1$ ,  $S_{1,\tilde{a}} = \tilde{k}_{1,\tilde{a}}^T \mu_a \simeq \mu_{1,\tilde{a}}^T \mu_a = 0$   
 $\alpha_{1,a} \simeq 1$ ,  $\alpha_{1,\tilde{a}} \simeq 0 \quad \therefore C_1 = \sum \alpha_{1,\tilde{a}} v_{\tilde{a}} \simeq v_a$   
 similarly,  $\alpha_{2,b} \simeq 1$ ,  $\alpha_{2,\tilde{a}} \simeq 0 \quad \therefore C_2 = \sum \alpha_{2,\tilde{a}} v_{\tilde{a}} \simeq v_b$   
 $C = \frac{1}{2}(C_1 + C_2) \simeq \frac{1}{2}(v_a + v_b)$

$$\Sigma_a = \alpha I + \frac{1}{2}(\mu_a \mu_a^T)$$

In head 1,  $\tilde{k}_a$  has the same direction with  $\mu_a$  and different magnitude.

so,  $C_1$  has a high variance and  $C_1$  becomes unstable.

While in head 2,  $\tilde{k}_a$  and  $\mu_b$  are orthogonal: the noise of  $\tilde{k}_a$  is negligible to  $C_2$ .

So  $C_2$  keeps close to  $v_b$  with low variance.

Finally,  $C = \frac{1}{2}(C_1 + C_2)$ , it makes its variance smaller than single-head attention